src/lib/utils/DY.Lib.Printing.fst
@@ -116,8 +116,8 @@ let rec usage_to_string u =
 /// in DY.Lib and DY.Core. This causes
 /// conflicts with the bytes_to_string function.
 
-val public_key_type_to_string: DY.Lib.State.PrivateKeys.public_key_type -> string
-let public_key_type_to_string t =
+val long_term_key_type_to_string: DY.Lib.State.PrivateKeys.long_term_key_type -> string
+let long_term_key_type_to_string t =
   match t with
   | DY.Lib.State.PrivateKeys.LongTermPkEncKey u -> "LongTermPkEncKey " ^ u
   | DY.Lib.State.PrivateKeys.LongTermSigKey u -> "LongTermSigKey " ^ u
@@ -129,7 +129,7 @@ let rec private_keys_types_to_string m =
   | [] -> ""
   | hd :: tl -> (
     (private_keys_types_to_string tl) ^ 
-    Printf.sprintf "%s = (%s)," (public_key_type_to_string hd.key.ty) (bytes_to_string hd.value.private_key)
+    Printf.sprintf "%s = (%s)," (long_term_key_type_to_string hd.key.ty) (bytes_to_string hd.value.private_key)
   )
 
 // The `#_` at the end is a workaround for FStarLang/FStar#3286
@@ -139,7 +139,7 @@ let rec pki_types_to_string m =
   | [] -> ""
   | hd :: tl -> (
     (pki_types_to_string tl) ^ 
-    Printf.sprintf "%s [%s] = (%s)," (public_key_type_to_string hd.key.ty) hd.key.who (bytes_to_string hd.value.public_key)
+    Printf.sprintf "%s [%s] = (%s)," (long_term_key_type_to_string hd.key.ty) hd.key.who (bytes_to_string hd.value.public_key)
   )
 
 val default_private_keys_state_to_string: bytes -> option string
