src/lib/state/DY.Lib.State.PKI.fst
@@ -26,7 +26,7 @@ open DY.Lib.State.PrivateKeys
 
 [@@ with_bytes bytes]
 type pki_key = {
-  ty:public_key_type;
+  ty:long_term_key_type;
   who:principal;
 }
 
@@ -71,12 +71,12 @@ val initialize_pki: prin:principal -> traceful state_id
 let initialize_pki = initialize_map pki_key pki_value #_ // another workaround for FStarLang/FStar#3286
 
 [@@ "opaque_to_smt"]
-val install_public_key: principal -> state_id -> public_key_type -> principal -> bytes -> traceful (option unit)
+val install_public_key: principal -> state_id -> long_term_key_type -> principal -> bytes -> traceful (option unit)
 let install_public_key prin sess_id pk_type who pk =
   add_key_value prin sess_id ({ty = pk_type; who;}) ({public_key = pk;})
 
 [@@ "opaque_to_smt"]
-val get_public_key: principal -> state_id -> public_key_type -> principal -> traceful (option bytes)
+val get_public_key: principal -> state_id -> long_term_key_type -> principal -> traceful (option bytes)
 let get_public_key prin sess_id pk_type who =
   let*? res = find_value prin sess_id ({ty = pk_type; who;}) in
   return (Some res.public_key)
@@ -101,7 +101,7 @@ let initialize_pki_invariant #invs prin tr =
 
 val install_public_key_invariant:
   {|protocol_invariants|} ->
-  prin:principal -> sess_id:state_id -> pk_type:public_key_type -> who:principal -> pk:bytes -> tr:trace ->
+  prin:principal -> sess_id:state_id -> pk_type:long_term_key_type -> who:principal -> pk:bytes -> tr:trace ->
   Lemma
   (requires
     is_public_key_for tr pk pk_type who /\
@@ -120,7 +120,7 @@ let install_public_key_invariant #invs prin sess_id pk_type who pk tr =
 
 val get_public_key_invariant:
   {|protocol_invariants|} ->
-  prin:principal -> sess_id:state_id -> pk_type:public_key_type -> who:principal -> tr:trace ->
+  prin:principal -> sess_id:state_id -> pk_type:long_term_key_type -> who:principal -> tr:trace ->
   Lemma
   (requires
     trace_invariant tr /\
